ObcToClight/DataflowElab.v
@@ -8,7 +8,12 @@ Require Import Rustre.ObcToClight.Interface.
 Require Import Rustre.Ident.
 
 Module Export OpAux := OperatorsAux Interface.Op.
+
+(* TODO: Tidy this up. Should just instantiate a Dataflow module to get
+         everything. *)
 Module Export Syn := SyntaxFun Ident.Ids Interface.Op.
+Module Export Mems := MemoriesFun Ident.Ids Interface.Op Syn.
+Module Export Defs := IsDefined Ident.Ids Interface.Op Syn Mems.
 
 Require Import List.
 Import List.ListNotations.
@@ -55,7 +60,27 @@ Module Type ELABORATION
 
   Section ElabExpressions.
 
+    (* Map variable names to types. *)
     Variable env : PM.t type.
+
+    (* Map variable names to clocks. *)
+    Variable cenv : PM.t clock.
+
+    (* Preceding dataflow program. *)
+    Variable G : global.
+
+    (* Map node names to input and output types. *)
+    Variable nenv : PM.t (list type * list type).
+
+    Hypothesis wt_cenv :
+      forall x ck, PM.find x cenv = Some ck -> wt_clock (PM.elements env) ck.
+
+    Hypothesis wt_nenv :
+      forall f n tysin tysout,
+        PM.find f nenv = Some (tysin, tysout) ->
+        (find_node f G = Some n
+         /\ Forall2 (fun i ty=> snd i = ty) n.(n_in) tysin
+         /\ Forall2 (fun i ty=> snd i = ty) [n.(n_out)] tysout).
 
     Definition find_type (loc: astloc) (x: ident) : res type :=
       match PM.find x env with
@@ -71,6 +96,30 @@ Module Type ELABORATION
                              :: MSG " but type " :: MSG (string_of_type ty)
                              :: MSG " was expected." :: nil)).
 
+    Definition find_clock (loc: astloc) (x: ident) : res clock :=
+      match PM.find x cenv with
+      | None => Error (err_loc loc (CTX x :: msg " is not declared."))
+      | Some ck => OK ck
+      end.
+
+    Definition find_node_interface (loc: astloc) (f: ident)
+                                              : res (list type * list type) :=
+      match PM.find f nenv with
+      | None => Error (err_loc loc (MSG "node " :: CTX f :: msg " not found."))
+      | Some tys => OK tys
+      end.
+
+    Lemma wt_find_clock:
+      forall loc x ck,
+        find_clock loc x = OK ck -> wt_clock (PM.elements env) ck.
+    Proof.
+      intros ** Hfind.
+      apply wt_cenv with (x:=x).
+      unfold find_clock in Hfind.
+      destruct (PM.find x cenv); try discriminate.
+      now monadInv Hfind.
+    Qed.
+    
     Fixpoint elab_clock (loc: astloc) (ck: Ast.clock) : res clock :=
       match ck with
       | BASE => OK Cbase
@@ -145,27 +194,27 @@ Module Type ELABORATION
       | VARIABLE sx loc =>
           let x := ident_of_string sx in
           do ty <- find_type loc x;
-          OK (Evar x ty)
+             OK (Evar x ty)
       | WHEN ae' b sx loc =>
           let x := ident_of_string sx in
           do ok <- assert_type loc x bool_type;
           do e' <- elab_lexp ae';
-          OK (Ewhen e' x b)
+             OK (Ewhen e' x b)
       | UNARY aop ae' loc =>
           let op := elab_unop aop in
           do e' <- elab_lexp ae';
           do ty' <- find_type_unop loc op (typeof e');
-          OK (Eunop op e' ty')
+             OK (Eunop op e' ty')
       | CAST aty' ae' loc =>
           let ty' := elab_type loc aty' in
           do e' <- elab_lexp ae';
-          OK (Eunop (CastOp ty') e' ty')
+             OK (Eunop (CastOp ty') e' ty')
       | BINARY aop ae1 ae2 loc =>
           let op := elab_binop aop in
           do e1 <- elab_lexp ae1;
           do e2 <- elab_lexp ae2;
           do ty' <- find_type_binop loc op (typeof e1) (typeof e2);
-          OK (Ebinop op e1 e2 ty')
+             OK (Ebinop op e1 e2 ty')
       | _ => Error (err_loc (expression_loc ae) (msg "expression not normalized"))
       end.
 
@@ -176,130 +225,344 @@ Module Type ELABORATION
         do ok <- assert_type loc x bool_type;
         do et <- elab_cexp aet;
         do ef <- elab_cexp aef;
-        if typeofc et ==b typeofc ef
-        then OK (Emerge x et ef)
-        else Error (err_loc loc (msg "badly typed merge"))
+           if typeofc et ==b typeofc ef
+           then OK (Emerge x et ef)
+           else Error (err_loc loc (msg "badly typed merge"))
       | IFTE ae aet aef loc =>
         do e <- elab_lexp ae;
         do et <- elab_cexp aet;
         do ef <- elab_cexp aef;
-        if (typeof e ==b bool_type) && (typeofc et ==b typeofc ef)
-        then OK (Eite e et ef)
-        else Error (err_loc loc (msg "badly typed if/then/else"))
+           if (typeof e ==b bool_type) && (typeofc et ==b typeofc ef)
+           then OK (Eite e et ef)
+           else Error (err_loc loc (msg "badly typed if/then/else"))
       | _ =>
         do e <- elab_lexp ae;
-        OK (Eexp e)
+           OK (Eexp e)
       end.
 
+    Definition assert_lexp_type (loc: astloc) (e: lexp) (ty: type) : res unit :=
+      if typeof e ==b ty then OK tt
+      else Error (err_loc loc (MSG "badly typed argument; expected "
+                                :: msg (string_of_type ty))).
+
+    Fixpoint elab_lexps (loc: astloc) (aes: list expression) (tys: list type)
+                                                            : res (list lexp) :=
+      match aes, tys with
+      | nil, nil => OK nil
+      | ae::aes, ty::tys =>
+          do e <- elab_lexp ae;
+          do ok <- assert_lexp_type (expression_loc ae) e ty;
+          do es <- elab_lexps loc aes tys;
+             OK (e::es)
+      | _, _ => Error (err_loc loc (msg "wrong number of arguments"))
+      end.
+
+    Fixpoint check_lists {A B} (loc: astloc) (f : A -> B -> res unit)
+                               (xs: list A) (ys: list B) : res unit :=
+      match xs, ys with
+      | nil, nil => OK tt
+      | x::xs, y::ys => do ok <- f x y; check_lists loc f xs ys
+      | _, _ => Error (err_loc loc (msg "wrong number of arguments"))
+      end.
+
+    Definition elab_equation (aeq: Ast.equation) : res equation :=
+      let '(sxs, ae, loc) := aeq in
+      do x <- match sxs with
+              | [sx] => OK (ident_of_string sx)
+              | _ => Error (err_loc loc
+                               (msg "multiple outputs not currently supported"))
+              end;
+      do ck <- find_clock loc x;
+      match ae with
+      | CALL sf aes loc =>
+        let f := ident_of_string sf in
+        do (tysin, tysout) <- find_node_interface loc f;
+        do es <- elab_lexps loc aes tysin;
+        do ok <- check_lists loc (assert_type loc) [x] tysout;
+        OK (EqApp x ck f es)
+
+      | FBY av0 ae loc =>
+        let v0 := elab_constant loc av0 in
+        let v0ty := type_const v0 in
+        do e <- elab_lexp ae;
+        do ok <- assert_type loc x v0ty;
+           if typeof e ==b v0ty
+           then OK (EqFby x ck v0 e)
+           else Error (err_loc loc (msg "badly typed fby"))
+
+      | _ =>
+        do e <- elab_cexp ae;
+        do ok <- assert_type loc x (typeofc e);
+           OK (EqDef x ck e)
+      end.
+
+    (** Properties *)
+    
+    Lemma find_type_In:
+      forall loc x ty,
+        find_type loc x = OK ty ->
+        In (x, ty) (PM.elements env).
+    Proof.
+      intros ** Hfty.
+      unfold find_type in Hfty.
+      destruct (PM.find x env) eqn:Hfind; try discriminate.
+      injection Hfty; intro; subst.
+      now apply PM.elements_correct in Hfind.
+    Qed.
+  
+    Lemma assert_type_In:
+      forall loc x ty y,
+        assert_type loc x ty = OK y ->
+        In (x, ty) (PM.elements env).
+    Proof.
+      intros loc x ty y Hhty.
+      unfold assert_type in Hhty.
+      monadInv Hhty.
+      destruct (x0 ==b ty) eqn:Heq.
+      2:discriminate EQ0.
+      rewrite equiv_decb_equiv in Heq.
+      rewrite Heq in *.
+      eauto using find_type_In.
+    Qed.
+    
+    Lemma wt_elab_clock:
+      forall loc ack ck,
+        elab_clock loc ack = OK ck ->
+        wt_clock (PM.elements env) ck.
+    Proof.
+      induction ack as [|ack IH]; simpl.
+      now injection 1; intro; subst; auto with dftyping.
+      intros ck Helab.
+      monadInv Helab.
+      constructor; auto.
+      apply assert_type_In with (1:=EQ).
+    Qed.
+
+    Lemma wt_elab_lexp:
+      forall ae e,
+        elab_lexp ae = OK e ->
+        wt_lexp (PM.elements env) e.
+    Proof.
+      induction ae; intros e Helab; monadInv Helab; constructor;
+        eauto using find_type_In, assert_type_In.
+      - unfold find_type_unop in EQ1.
+        rewrite type_unop'_correct in EQ1.
+        now DestructCases.
+      - unfold find_type_binop in EQ0.
+        match goal with H:match ?e with _ => _ end = _ |- _ =>
+          destruct e eqn:He; try discriminate; injection H end.
+        intro; subst.
+        now rewrite type_binop'_correct in He.
+      - now rewrite type_castop.
+    Qed.
+
+    Lemma wt_elab_cexp:
+      forall ae e,
+        elab_cexp ae = OK e ->
+        wt_cexp (PM.elements env) e.
+    Proof.
+      induction ae; intros e Helab.
+      - apply bind_inversion in Helab.
+        destruct Helab as (le & Helab & Hexp).
+        monadInv Hexp. eauto using wt_elab_lexp with dftyping.
+      - apply bind_inversion in Helab.
+        destruct Helab as (le & Helab & Hexp).
+        monadInv Hexp. eauto using wt_elab_lexp with dftyping.
+      - monadInv Helab.
+        specialize (IHae2 _ EQ1); clear EQ1.
+        specialize (IHae3 _ EQ0); clear EQ0.
+        destruct ((typeof x ==b bool_type) && (typeofc x0 ==b typeofc x1)) eqn:Hg;
+          try discriminate.
+        apply andb_prop in Hg; destruct Hg as (Hg1 & Hg2).
+        rewrite equiv_decb_equiv in Hg1, Hg2.
+        monadInv EQ3. eauto using wt_elab_lexp with dftyping.
+      - apply bind_inversion in Helab.
+        destruct Helab as (le & Helab & Hexp).
+        monadInv Hexp. eauto using wt_elab_lexp with dftyping.
+      - apply bind_inversion in Helab.
+        destruct Helab as (le & Helab & Hexp).
+        monadInv Hexp. eauto using wt_elab_lexp with dftyping.
+      - apply bind_inversion in Helab.
+        destruct Helab as (le & Helab & Hexp).
+        monadInv Hexp. eauto using wt_elab_lexp with dftyping.
+      - apply bind_inversion in Helab.
+        destruct Helab as (le & Helab & Hexp).
+        monadInv Hexp. eauto using wt_elab_lexp with dftyping.
+      - apply bind_inversion in Helab.
+        destruct Helab as (le & Helab & Hexp).
+        monadInv Hexp. eauto using wt_elab_lexp with dftyping.
+      - apply bind_inversion in Helab.
+        destruct Helab as (le & Helab & Hexp).
+        monadInv Hexp. eauto using wt_elab_lexp with dftyping.
+      - monadInv Helab.
+        specialize (IHae1 _ EQ1); clear EQ1.
+        specialize (IHae2 _ EQ0); clear EQ0.
+        destruct ((typeofc x0 ==b typeofc x1)) eqn:Hg;
+          try discriminate.
+        rewrite equiv_decb_equiv in Hg.
+        monadInv EQ3. apply assert_type_In in EQ.
+        auto with dftyping.
+    Qed.
+
+    Lemma wt_elab_equation:
+      forall aeq eq,
+        elab_equation aeq = OK eq ->
+        wt_equation G (PM.elements env) eq.
+    Proof.
+      intros aeq eq Helab.
+      destruct aeq as ((xs & ae) & loc).
+      destruct ae; simpl in Helab;
+        repeat progress
+               match goal with H:bind _ _ = _ |- _ => monadInv H end.
+      - admit.
+      - admit.
+      - admit.
+      - admit.
+      - admit.
+      - admit.
+      - admit.
+      - admit.
+      - admit.
+      - admit.
+    Qed.
+    
   End ElabExpressions.
 
-  Lemma find_type_In:
-    forall env loc x ty,
-      find_type env loc x = OK ty ->
-      In (x, ty) (PM.elements env).
-  Proof.
-    intros ** Hfty.
-    unfold find_type in Hfty.
-    destruct (PM.find x env) eqn:Hfind; try discriminate.
-    injection Hfty; intro; subst.
-    now apply PM.elements_correct in Hfind.
-  Qed.
-  
-  Lemma assert_type_In:
-    forall env loc x ty y,
-      assert_type env loc x ty = OK y ->
-      In (x, ty) (PM.elements env).
-  Proof.
-    intros env loc x ty y Hhty.
-    unfold assert_type in Hhty.
-    monadInv Hhty.
-    destruct (x0 ==b ty) eqn:Heq.
-    2:discriminate EQ0.
-    rewrite equiv_decb_equiv in Heq.
-    rewrite Heq in *.
-    eauto using find_type_In.
-  Qed.
-    
-  Lemma wt_elab_clock:
-    forall env loc ack ck,
-      elab_clock env loc ack = OK ck ->
-      wt_clock (PM.elements env) ck.
-  Proof.
-    induction ack as [|ack IH]; simpl.
-    now injection 1; intro; subst; auto with dftyping.
-    intros ck Helab.
-    monadInv Helab.
-    constructor; auto.
-    apply assert_type_In with (1:=EQ).
-  Qed.
+  Section ElabDeclaration.
 
-  Lemma wt_elab_lexp:
-    forall env ae e,
-      elab_lexp env ae = OK e ->
-      wt_lexp (PM.elements env) e.
-  Proof.
-    induction ae; intros e Helab; monadInv Helab; constructor;
-      eauto using find_type_In, assert_type_In.
-    - unfold find_type_unop in EQ1.
-      rewrite type_unop'_correct in EQ1.
-      now DestructCases.
-    - unfold find_type_binop in EQ0.
-      match goal with H:match ?e with _ => _ end = _ |- _ =>
-        destruct e eqn:He; try discriminate; injection H end.
-      intro; subst.
-      now rewrite type_binop'_correct in He.
-    - now rewrite type_castop.
-  Qed.
+    (* Preceding dataflow program. *)
+    Variable G : global.
 
-  Lemma wt_elab_cexp:
-    forall env ae e,
-      elab_cexp env ae = OK e ->
-      wt_cexp (PM.elements env) e.
-  Proof.
-    induction ae; intros e Helab.
-    - apply bind_inversion in Helab.
-      destruct Helab as (le & Helab & Hexp).
-      monadInv Hexp. eauto using wt_elab_lexp with dftyping.
-    - apply bind_inversion in Helab.
-      destruct Helab as (le & Helab & Hexp).
-      monadInv Hexp. eauto using wt_elab_lexp with dftyping.
-    - monadInv Helab.
-      specialize (IHae2 _ EQ1); clear EQ1.
-      specialize (IHae3 _ EQ0); clear EQ0.
-      destruct ((typeof x ==b bool_type) && (typeofc x0 ==b typeofc x1)) eqn:Hg;
-        try discriminate.
-      apply andb_prop in Hg; destruct Hg as (Hg1 & Hg2).
-      rewrite equiv_decb_equiv in Hg1, Hg2.
-      monadInv EQ3. eauto using wt_elab_lexp with dftyping.
-    - apply bind_inversion in Helab.
-      destruct Helab as (le & Helab & Hexp).
-      monadInv Hexp. eauto using wt_elab_lexp with dftyping.
-    - apply bind_inversion in Helab.
-      destruct Helab as (le & Helab & Hexp).
-      monadInv Hexp. eauto using wt_elab_lexp with dftyping.
-    - apply bind_inversion in Helab.
-      destruct Helab as (le & Helab & Hexp).
-      monadInv Hexp. eauto using wt_elab_lexp with dftyping.
-    - apply bind_inversion in Helab.
-      destruct Helab as (le & Helab & Hexp).
-      monadInv Hexp. eauto using wt_elab_lexp with dftyping.
-    - apply bind_inversion in Helab.
-      destruct Helab as (le & Helab & Hexp).
-      monadInv Hexp. eauto using wt_elab_lexp with dftyping.
-    - apply bind_inversion in Helab.
-      destruct Helab as (le & Helab & Hexp).
-      monadInv Hexp. eauto using wt_elab_lexp with dftyping.
-    - monadInv Helab.
-      specialize (IHae1 _ EQ1); clear EQ1.
-      specialize (IHae2 _ EQ0); clear EQ0.
-      destruct ((typeofc x0 ==b typeofc x1)) eqn:Hg;
-        try discriminate.
-      rewrite equiv_decb_equiv in Hg.
-      monadInv EQ3. apply assert_type_In in EQ.
-      auto with dftyping.
-  Qed.
+    (* Map node names to input and output types. *)
+    Variable nenv : PM.t (list type * list type).
 
+    Hypothesis wt_nenv :
+      forall f n tysin tysout,
+        PM.find f nenv = Some (tysin, tysout) ->
+        (find_node f G = Some n
+         /\ Forall2 (fun i ty=> snd i = ty) n.(n_in) tysin
+         /\ Forall2 (fun i ty=> snd i = ty) [n.(n_out)] tysout).
+
+    Definition elab_var_decl (acc: list (ident * type) * (PS.t * PM.t type))
+               (vd: string * type_name * Ast.clock * astloc)
+               : (list (ident * type) * (PS.t * PM.t type)) :=
+      let '(rs, (vars, tyenv)) := acc in
+      let '(sx, sty, sck, loc) := vd in
+      let x := ident_of_string sx in
+      let ty := elab_type loc sty in
+      ((x, ty)::rs, (PS.add x vars, PM.add x ty tyenv)).
+
+    Fixpoint check_defd (out: PS.t) (defd: PS.t) (eqs: list equation) : bool :=
+      match eqs with
+      | nil => PS.is_empty defd
+      | eq::eqs => let x := var_defined eq in
+                   if PS.mem x defd && (negb (is_fby eq && PS.mem x out))
+                   then check_defd out (PS.remove x defd) eqs
+                   else false
+      end.
+
+    Fixpoint elab_clock_decl (tyenv: PM.t type) (acc: PM.t clock)
+               (vds: list (string * type_name * Ast.clock * astloc))
+               : res (PM.t clock) :=
+      match vds with
+      | nil => OK acc
+      | vd::vds =>
+        let '(sx, sty, sck, loc) := vd in
+        let x := ident_of_string sx in
+        do ck <- elab_clock tyenv loc sck;
+           elab_clock_decl tyenv (PM.add x ck acc) vds
+      end.
+
+    Program Definition elab_declaration (nenv: PM.t (list type * list type))
+                                        (decl: Ast.declaration) : res node :=
+      match decl with
+      | NODE name inputs outputs locals equations loc =>
+        let '(xout, sout) := fold_left elab_var_decl outputs
+                                       ([], (PS.empty, PM.empty type)) in
+        let '(xlocal, svars) := fold_left elab_var_decl locals ([], sout) in
+        let '(xin, (allvars, tyenv)) := fold_left elab_var_decl inputs
+                                                  ([], svars) in
+        match elab_clock_decl tyenv (PM.empty clock)
+                              (inputs ++ outputs ++ locals) with
+        | OK ckenv =>
+          match mmap (elab_equation tyenv ckenv nenv) equations with
+          | OK eqs =>
+            match check_defd (fst sout) (fst (svars)) eqs with
+            | false => Error (err_loc loc (msg "a variable is not properly defined"))
+            | true =>
+              match existsb (fun x=>PS.mem x allvars) Ident.Ids.reserved with
+              | true => Error (err_loc loc (msg "illegal variable name"))
+              | false =>
+                match length xin ==b 0 with
+                | true => Error (err_loc loc (msg "not enough inputs"))
+                | false =>
+                  match xout with
+                  | o::nil => OK {| n_name  := ident_of_string name;
+                                    n_in    := xin;
+                                    n_out   := o;
+                                    n_vars  := xlocal;
+                                    n_eqs   := eqs;
+                                    n_ingt0 := _;
+                                    n_defd  := _;
+                                    n_vout  := _;
+                                    n_nodup := _;
+                                    n_good  := _ |}
+                  | _ => Error (err_loc loc (msg "need one output"))
+                  end
+                end
+              end
+            end
+          | Error e => Error e
+          end
+        | Error e => Error e
+        end
+      end.
+    Next Obligation.
+      (* 0 < length xin *)
+      match goal with H:false = (length xin ==b 0) |- _ => rename H into Hin end.
+      symmetry in Hin. apply not_equiv_decb_equiv in Hin.
+      now apply NPeano.Nat.neq_0_lt_0 in Hin.
+    Qed.
+    Next Obligation.
+      (* Permutation (map var_defined eqs) (map fst (xlocal ++ [(i, t)])) *)
+      admit.
+    Qed.
+    Next Obligation.
+      (* ~ In (fst (i, t)) (map var_defined (filter is_fby eqs)) *)
+      admit.
+    Qed.
+    Next Obligation.
+      (* NoDupMembers (xin ++ xlocal ++ [(i, t)]) *)
+      admit.
+    Qed.
+    Next Obligation.
+      (* Forall NotReserved (xin ++ xlocal ++ [(i, t)]) *)
+      match goal with H:context [PS.mem _ allvars] |- _ => rename H into Hr end.
+      symmetry in Hr.
+      admit.
+    Qed.
+
+  End ElabDeclaration.
+
+  Fixpoint elab_declarations' (nenvg: PM.t (list type * list type) * global)
+                              (decls: list Ast.declaration) : res global :=
+    let (nenv, g) := nenvg in
+    match decls with
+    | nil => OK g
+    | d::ds =>
+      do n <- elab_declaration nenv d;
+         let loc := declaration_loc d in
+         if find_node_interface nenv loc n.(n_name)
+         then Error (err_loc loc (MSG "duplicate definition for "
+                                      :: CTX n.(n_name) :: nil))
+         else elab_declarations'
+                (PM.add n.(n_name) (map snd n.(n_in),
+                                    map snd [n.(n_out)]) nenv, n :: g) ds
+    end.
+
+  Definition elab_declarations (decls: list Ast.declaration) : res global :=
+    elab_declarations' (PM.empty (list type * list type), []) decls.
+           
 End ELABORATION.
-
 
 
